Working on App for inference

inference/proofs/inferCompleteScript.sml
@@ -37,14 +37,23 @@ val unconvert_t_def = tDefine "unconvert_t" `
  full_simp_tac (srw_ss()++ARITH_ss) []);
 
 val tenv_inv_def = Define `
-tenv_inv s env tenv =
+tenv_inv s tenv tenvE =
   (!x tvs t.
-    lookup_tenv x 0 tenv = SOME (tvs, t)
+    lookup_tenv x 0 tenvE = SOME (tvs, t)
     ⇒
-    check_freevars tvs [] t ∧
-    ?t'. unconvert_t t = t_walkstar s t' ∧ 
-         (tvs > 0 ⇒ t_walkstar s t' = t') ∧ 
-	 ALOOKUP env x = SOME (tvs,t'))`;
+    (*tvs >0 ⇒ check_freevars (num_tvs tenvE) [] t ∧ *)
+    (if tvs > 0 then check_freevars tvs [] t
+                else ?n.check_freevars n [] t) ∧
+    ?t'.
+    unconvert_t t = t_walkstar s t' ∧ 
+    (tvs > 0 ⇒ t_walkstar s t' = t') ∧
+    (*
+    (!targs. LENGTH targs ≤ tvs
+    ⇒ 
+    infer_deBruijn_subst targs (unconvert_t t) = 
+    infer_deBruijn_subst targs (t_walkstar s t')) ∧ *)
+
+    ALOOKUP tenv x = SOME (tvs,t'))`;
 
 
 val t_walk_vwalk_id = prove
@@ -229,10 +238,10 @@ val new_uvars_sub_completion_exists = Q.prove (
 (*Ignore increment on deBrujin vars*)
 val t_walkstar_ignore_inc = prove(
 ``t_wfs s ⇒ 
-(!t.(!uv. uv ∈ FDOM s ⇒ check_t k {} (t_walkstar s (Infer_Tuvar uv)))
+(!t.(!uv. uv ∈ FDOM s ⇒ check_t 0 {} (t_walkstar s (Infer_Tuvar uv)))
 ⇒
 t_walkstar (infer_deBruijn_inc tvs o_f s) t = t_walkstar s t) ∧
-(!ts. (!t.(!uv. uv ∈ FDOM s ⇒ check_t k {} (t_walkstar s (Infer_Tuvar uv)))
+(!ts. (!t.(!uv. uv ∈ FDOM s ⇒ check_t 0 {} (t_walkstar s (Infer_Tuvar uv)))
 ⇒
 EVERY (\t. t_walkstar (infer_deBruijn_inc tvs o_f s) t = t_walkstar s t) ts))``, 
   strip_tac>>
@@ -258,49 +267,6 @@ EVERY (\t. t_walkstar (infer_deBruijn_inc tvs o_f s) t = t_walkstar s t) ts))``,
   fs[infer_deBruijn_inc_def])
 
 
-val debruijn_subst_infer_deBruijn_inc_ignore = prove(
-``
-t_wfs s ∧ 
-(!uv. uv ∈ FDOM s ⇒ check_t n {} (t_walkstar s (Infer_Tuvar uv)))
-⇒
-(!t' t.
-convert_t (t_walkstar s t') = t 
-⇒ 
-deBruijn_subst 0 ls t = 
-deBruijn_subst 0 ls (convert_t (t_walkstar (infer_deBruijn_inc (LENGTH ls) o_f s) t'))) ∧ 
-(!ts' ts. 
-ts = MAP (convert_t o (t_walkstar s)) ts'
-⇒
-MAP (deBruijn_subst 0 ls) ts =
-MAP (deBruijn_subst 0 ls) 
-    (MAP (convert_t o (t_walkstar(infer_deBruijn_inc (LENGTH ls) o_f s))) ts'))``
-
-strip_tac>>
-ho_match_mp_tac infer_tTheory.infer_t_induction>>
-imp_res_tac inc_wfs>>
-rpt strip_tac>>fs[]
->-
-  fs[t_walkstar_eqn1,convert_t_def,EQ_SYM_EQ]
->-
-  (pop_assum mp_tac>>
-  fs[t_walkstar_eqn1,convert_t_def,EQ_SYM_EQ,MAP_EQ_ID]>>
-  fs[deBruijn_subst_def,MAP_MAP_o,MAP_EQ_f]>>
-  rw[] 
-  )
->>
-  fs[walkstar_inc2,convert_inc]>>
-  Cases_on`n' ∈ FDOM s`>> (*dont need cases*)
-  >-
-    res_tac>>
-    imp_res_tac convert_inc>>
-    pop_assum (qspec_then `LENGTH ls` SUBST1_TAC)>>
-    qpat_abbrev_tac `t' = convert_t A`>>
-    assume_tac (fst (CONJ_PAIR subst_inc_cancel))>>
-    pop_assum(qspecl_then [`t`,`ls`,`0`] assume_tac)>>
-    fs[]
-    
-    de
-    pop_assum(qspecl_then [`t`,`
 (*Adding a list of keys that did not already exist is safe*)
 val SUBMAP_FUPDATE_LIST_NON_EXIST = prove(
 ``set (MAP FST ls) ∩ (FDOM s) = {} 
@@ -353,6 +319,99 @@ val t_walkstar_o_f_id = prove(
   fs[MAP_EQ_f]>>rw[]>>res_tac>>
   fs[t_walkstar_eqn])
 
+val deBruijn_subst_id = prove(
+``(!t. deBruijn_subst 0 [] t = t) ∧
+  (!ts. MAP (deBruijn_subst 0 []) ts = ts)``,
+  Induct>>rw[]>>fs[deBruijn_subst_def,MAP_EQ_ID])
+
+val infer_deBruijn_subst_id = prove(
+``(!t. infer_deBruijn_subst [] t = t) ∧ 
+  (!ts. MAP (infer_deBruijn_subst []) ts = ts)``,
+  Induct>>rw[]>>fs[infer_deBruijn_subst_def,MAP_EQ_ID])
+
+val tenv_inv_submap = prove(
+``s SUBMAP s' ∧
+  t_wfs s' ∧ 
+  tenv_inv s tenv tenvE ⇒ 
+  tenv_inv s' tenv tenvE``,
+  rw[tenv_inv_def]
+  >-
+    metis_tac[] 
+  >>
+    res_tac>>
+    `t_walkstar s t' = t_walkstar s' t'` by
+      (imp_res_tac t_walkstar_SUBMAP>>
+      pop_assum(qspec_then`t'` SUBST1_TAC)>>
+      Cases_on`tvs`>>
+      metis_tac[check_freevars_to_check_t,t_walkstar_no_vars])>>
+    fs[])
+
+
+(*Constraints are strong enough to ignore the unification*)
+(*val t_unify... = prove
+``(!t. t_walkstar s h = t ∧ check_t tvs {} t ∧ t_wfs st.subst ∧  
+  sub_completion n st.next_uvar st.subst constraints s 
+  ⇒ 
+  ?n_subst.
+    t_unify st.subst h t = SOME n_subst ∧ 
+    sub_completion n st.next_uvar n_subst constraints s) ∧ 
+  (!ts. MAP (t_walkstar s) hs = ts ∧ EVERY (check_t tvs {}) ts ∧  t_wfs st.subst ∧ 
+  sub_completion n st.next_uvar st.subst constraints s
+  ⇒
+  ?n_subst.
+    ts_unify st.subst hs ts = SOME n_subst ∧
+    sub_completion n st.next_uvar n_subst constraints s)``
+  
+  Induct>>
+  >-
+    ntac 2 strip_tac>>
+    imp_res_tac sub_completion_wfs>>
+    Cases_on`h`>>
+    fs[t_walkstar_eqn,t_walk_eqn,t_unify_eqn,t_ext_s_check_eqn]
+    BasicProvers.FULL_CASE_TAC>>
+    (*Lemma here to invert sub_completion:
+    if st subcompletes to s and t_vwalk on s is Infer_Tvar_db,
+    then t_vwalk on st must either be Infer_Tvar_db OR Tuvar.
+
+    *)
+  >-
+    strip_tac>>
+    fs[t_walkstar_eqn]
+  Cases_on`t`>>
+
+val constrain_op_complete = prove
+``
+!n. 
+type_op op (MAP (convert_t o t_walkstar s) ts) t ∧ 
+sub_completion n st.next_uvar st.subst constraints s ∧ 
+FDOM st.subst ⊆ count st.next_uvar ∧ 
+FDOM s = count st.next_uvar ∧
+t_wfs st.subst 
+⇒
+?t' st' s' constraints'.
+constrain_op op ts st = (Success t',st') ∧
+sub_completion n st'.next_uvar st'.subst constraints' s' ∧
+s SUBMAP s' ∧
+FDOM st'.subst ⊆ count st'.next_uvar ∧  
+FDOM s' = count st'.next_uvar ∧ 
+t = convert_t (t_walkstar s' t')``,
+strip_tac>>
+fs[constrain_op_def,type_op_cases]>>
+BasicProvers.EVERY_CASE_TAC>>
+fs[success_eqns,constrain_op_success]>>rw[]
+>-
+  Q.EXISTS_TAC`Infer_Tapp [] TC_int`>>
+  fs[Once SWAP_EXISTS_THM]>>
+  Q.
+  fs[t_walkstar_eqn]
+
+
+(Cases_on`ts = []`>>fs[]>>
+ Cases_on`ts = [)
+
+fs[success_eqns]
+*)
+
 val infer_e_complete = Q.prove (
 
 `(!tenvM tenvC tenvE e t. 
@@ -364,6 +423,7 @@ val infer_e_complete = Q.prove (
      sub_completion (num_tvs tenvE) st.next_uvar st.subst constraints s ∧
      (*I think these conditions are reasonable... the second one maybe not*)
      FDOM st.subst ⊆ count st.next_uvar ∧ 
+     (*This constrains constraints to only constrain the necessary unification variables*)
      FDOM s = count st.next_uvar ∧
      tenv_inv s tenv tenvE
      ⇒
@@ -371,7 +431,8 @@ val infer_e_complete = Q.prove (
        infer_e menv tenvC tenv e st = (Success t', st') ∧
        sub_completion (num_tvs tenvE) st'.next_uvar st'.subst constraints' s' ∧
        FDOM st'.subst ⊆  count st'.next_uvar ∧ 
-       FDOM s' = count st'.next_uvar ∧ 
+       FDOM s' = count st'.next_uvar ∧
+       s SUBMAP s' ∧   
        t = convert_t (t_walkstar s' t')) ∧
  (!tenvM tenvC tenvE es ts. 
    type_es tenvM tenvC tenvE es ts
@@ -379,12 +440,17 @@ val infer_e_complete = Q.prove (
    !s menv tenv st constraints.
      tenvM = convert_menv menv ∧
      t_wfs st.subst ∧
-     sub_completion 0 st.next_uvar st.subst constraints s ∧
+     sub_completion (num_tvs tenvE) st.next_uvar st.subst constraints s ∧
+     FDOM st.subst ⊆ count st.next_uvar ∧ 
+     FDOM s = count st.next_uvar ∧ 
      tenv_inv s tenv tenvE
      ⇒
      ?ts' st' s' constraints'.
        infer_es menv tenvC tenv es st = (Success ts', st') ∧
        sub_completion 0 st'.next_uvar st'.subst constraints' s' ∧
+       FDOM st'.subst ⊆ count st'.next_uvar ∧ 
+       FDOM s' = count st'.next_uvar ∧ 
+       s SUBMAP s' ∧ 
        ts = MAP (convert_t o t_walkstar s') ts') ∧
  (!tenvM tenvC tenvE funs env. 
    type_funs tenvM tenvC tenvE funs env
@@ -392,12 +458,17 @@ val infer_e_complete = Q.prove (
    !s menv tenv st constraints.
      tenvM = convert_menv menv ∧
      t_wfs st.subst ∧
-     sub_completion 0 st.next_uvar st.subst constraints s ∧
+     sub_completion (num_tvs tenvE) st.next_uvar st.subst constraints s ∧
+     FDOM st.subst ⊆ count st.next_uvar ∧ 
+     FDOM s = count st.next_uvar ∧ 
      tenv_inv s tenv tenvE
      ⇒
      ?env' st' s' constraints'.
        infer_funs menv tenvC tenv funs st = (Success env', st') ∧
        sub_completion 0 st'.next_uvar st'.subst constraints' s' ∧
+       FDOM st'.subst ⊆ count st'.next_uvar ∧ 
+       FDOM s' = count st'.next_uvar ∧
+       s SUBMAP s' ∧  
        MAP SND env = MAP (convert_t o t_walkstar s') env')`,
  ho_match_mp_tac type_e_strongind >>
  rw [success_eqns,infer_e_def]
@@ -491,8 +562,14 @@ val infer_e_complete = Q.prove (
          rw [success_eqns] >>
          rw [Once SWAP_EXISTS_THM] >>
 	 qexists_tac `constraints++(ZIP 
-	   (MAP (λn. Infer_Tuvar (st.next_uvar + n)) (COUNT_LIST (LENGTH targs))
-           ,MAP unconvert_t targs))` >>
+	 (MAP (λn. Infer_Tuvar (st.next_uvar + n)) (COUNT_LIST (LENGTH targs))
+         ,MAP unconvert_t targs))`>>
+	 (*	 qexists_tac `
+		 MAP (λ k,v. 
+		   let s = MAP unconvert_t targs in 
+		   infer_deBruijn_subst s k, infer_deBruijn_subst s v) constraints++(ZIP 
+		   (MAP (λn. Infer_Tuvar (st.next_uvar + n)) (COUNT_LIST (LENGTH targs))
+		   ,MAP unconvert_t targs))` >>*)
          `t_wfs s` by metis_tac[sub_completion_wfs]>>
 	 fs[sub_completion_def,pure_add_constraints_append]>>
 	 fs[PULL_EXISTS,Once SWAP_EXISTS_THM]>>
@@ -574,71 +651,220 @@ val infer_e_complete = Q.prove (
 	   fs[MEM_COUNT_LIST]>>
 	   DECIDE_TAC)>>
 	(*deBruijn_subst*)
-	 assume_tac (db_subst_infer_subst_swap|>CONJ_PAIR|>fst)>>
-	 pop_assum (qspecl_then [`t'`,`s'`,`LENGTH targs`
-	                        ,`st.next_uvar`,`num_tvs tenvE`] assume_tac)>>
-	 `check_t (LENGTH targs) (FDOM s') t'` by
-	  (imp_res_tac check_t_t_walkstar>>
-	   `FDOM s ⊆ FDOM s'` by 
-	     fs[Abbr`s'`,FDOM_FUPDATE_LIST]>> 
-	   imp_res_tac check_t_more5)>> 
-	 rfs[check_t_more]>>
-	 fs[MAP_MAP_o]>>
-         `(MAP (convert_t o t_walkstar s' o (λn. Infer_Tuvar (st.next_uvar + n)))
-               (COUNT_LIST (LENGTH targs))) = targs` by
-	 (
-	 match_mp_tac LIST_EQ>>
-	 fs[LENGTH_COUNT_LIST]>>rw[]>>
-	 fs[EL_MAP,LENGTH_COUNT_LIST,EL_COUNT_LIST]>>
-	 qpat_abbrev_tac `tar = EL x targs`>>
-	 fs[t_walkstar_eqn,t_walk_eqn,Once t_vwalk_eqn]>>
-	 `FLOOKUP s' (st.next_uvar +x) = SOME (unconvert_t tar)` by
-	 (
-	   fs[Abbr`s'`,flookup_update_list_some]>>DISJ1_TAC>>
-           qmatch_abbrev_tac `ALOOKUP (REVERSE L) k = SOME Y`>>
-	   Q.ISPECL_THEN [`L`,`k`] mp_tac alookup_distinct_reverse>>
-	   `ALL_DISTINCT (MAP FST L)` by
-	   (rw[Abbr`L`,MAP_ZIP,LENGTH_COUNT_LIST]>>
-	    match_mp_tac ALL_DISTINCT_MAP_INJ>>
-	    fs[all_distinct_count_list])>>
-	    rw[]>>
-	    unabbrev_all_tac>>
-	    match_mp_tac ALOOKUP_ALL_DISTINCT_MEM>>fs[]>>
-	    fs[MEM_ZIP,LENGTH_COUNT_LIST]>>HINT_EXISTS_TAC>>
-	    fs[EL_MAP,LENGTH_COUNT_LIST,EL_COUNT_LIST])>>
-	  fs[]>>
-	  fs[EVERY_EL]>>last_x_assum(qspec_then `x` assume_tac)>>
-	  rfs[]>>
-	  imp_res_tac check_freevars_to_check_t>>
-	  imp_res_tac check_freevars_empty_convert_unconvert_id>>
-	  Cases_on`unconvert_t tar`
-	  >-
-	    (fs[]>>metis_tac[])
-	  >-
-	    (fs[check_t_def]>>
-	    `MAP (t_walkstar s') l = l` by
-	      (fs[MAP_EQ_ID,EVERY_MEM]>>rw[]>>
-	      metis_tac[t_walkstar_no_vars])>>fs[])
-	  >>
-	    fs[check_t_def])>>
-	 fs[]>>
-	 Cases_on`LENGTH targs >0`
+	 reverse (Cases_on`LENGTH targs >0`)
 	 >-
-	   (fs[]>>
-	   imp_res_tac inc_wfs>>
-	   AP_TERM_TAC>>
-	   metis_tac[t_walkstar_no_vars,check_freevars_empty_convert_unconvert_id])
-	 >>
-	   `LENGTH targs = 0` by DECIDE_TAC>>
-	   fs[t_walkstar_o_f_id]>>
+	   (`LENGTH targs = 0` by DECIDE_TAC>>
+	   fs[LENGTH_NIL,deBruijn_subst_id,COUNT_LIST_def,infer_deBruijn_subst_id]>>
 	   `t_walkstar s' t' = t_walkstar s t'` by
 	     (imp_res_tac t_walkstar_SUBMAP>>
 	     first_x_assum(qspec_then `t'` mp_tac)>>
-	     rw[]>>metis_tac[t_walkstar_no_vars])>>
-	   metis_tac[check_freevars_empty_convert_unconvert_id])
+	     imp_res_tac check_freevars_to_check_t>>
+	     rw[]>>metis_tac[t_walkstar_no_vars])>> 
+	    pop_assum SUBST_ALL_TAC>>
+	    qpat_assum `unconvert_t t = bla` (assume_tac o Q.AP_TERM `convert_t`)>>
+	    metis_tac[check_freevars_empty_convert_unconvert_id])
+	 >>
+	   fs[]>>
+	   imp_res_tac check_freevars_to_check_t>>
+	   assume_tac (db_subst_infer_subst_swap|>CONJ_PAIR|>fst)>>
+	   pop_assum (qspecl_then [`t'`,`s'`,`LENGTH targs`
+	                        ,`st.next_uvar`,`num_tvs tenvE`] assume_tac)>>
+	   `check_t (LENGTH targs) (FDOM s') t'` by
+	    (imp_res_tac check_t_t_walkstar>>
+	     `FDOM s ⊆ FDOM s'` by 
+	       fs[Abbr`s'`,FDOM_FUPDATE_LIST]>> 
+	     imp_res_tac check_t_more5>>
+	     metis_tac[EMPTY_SUBSET])>> 
+	   rfs[check_t_more]>>
+	   fs[MAP_MAP_o]>>
+           `(MAP (convert_t o t_walkstar s' o (λn. Infer_Tuvar (st.next_uvar + n)))
+                 (COUNT_LIST (LENGTH targs))) = targs` by
+	   (
+	   match_mp_tac LIST_EQ>>
+	   fs[LENGTH_COUNT_LIST]>>rw[]>>
+	   fs[EL_MAP,LENGTH_COUNT_LIST,EL_COUNT_LIST]>>
+	   qpat_abbrev_tac `tar = EL x targs`>>
+	   fs[t_walkstar_eqn,t_walk_eqn,Once t_vwalk_eqn]>>
+	   `FLOOKUP s' (st.next_uvar +x) = SOME (unconvert_t tar)` by
+	   (
+	     fs[Abbr`s'`,flookup_update_list_some]>>DISJ1_TAC>>
+             qmatch_abbrev_tac `ALOOKUP (REVERSE L) k = SOME Y`>>
+	     Q.ISPECL_THEN [`L`,`k`] mp_tac alookup_distinct_reverse>>
+	     `ALL_DISTINCT (MAP FST L)` by
+	     (rw[Abbr`L`,MAP_ZIP,LENGTH_COUNT_LIST]>>
+	      match_mp_tac ALL_DISTINCT_MAP_INJ>>
+	      fs[all_distinct_count_list])>>
+	     rw[]>>
+	     unabbrev_all_tac>>
+	     match_mp_tac ALOOKUP_ALL_DISTINCT_MEM>>fs[]>>
+	     fs[MEM_ZIP,LENGTH_COUNT_LIST]>>HINT_EXISTS_TAC>>
+	     fs[EL_MAP,LENGTH_COUNT_LIST,EL_COUNT_LIST])>>
+	   fs[]>>
+	   fs[EVERY_EL]>>last_x_assum(qspec_then `x` assume_tac)>>
+	   rfs[]>>
+	   imp_res_tac check_freevars_to_check_t>>
+	   imp_res_tac check_freevars_empty_convert_unconvert_id>>
+	   Cases_on`unconvert_t tar`
+	   >-
+	     (fs[]>>metis_tac[])
+	   >-
+	     (fs[check_t_def]>>
+	     `MAP (t_walkstar s') l = l` by
+	       (fs[MAP_EQ_ID,EVERY_MEM]>>rw[]>>
+	       metis_tac[t_walkstar_no_vars])>>fs[])
+	   >>
+	     fs[check_t_def])>>
+	 fs[]>>
+	 imp_res_tac inc_wfs>>
+	 AP_TERM_TAC>>
+	 metis_tac[t_walkstar_no_vars,check_freevars_empty_convert_unconvert_id])
     >-
     (*Long*)
     cheat)
+ >-
+   (*Fun*)
+   (fs[bind_tenv_def,num_tvs_def,tenv_inv_def]>>
+   Q.ABBREV_TAC `constraints' = constraints++
+                 [Infer_Tuvar st.next_uvar,unconvert_t t1]`>>
+   imp_res_tac pure_add_constraints_exists>>
+   pop_assum (qspecl_then [`[t1]`,`num_tvs tenvE`] mp_tac)>>
+   miscLib.discharge_hyps>>fs[]>>
+   miscLib.discharge_hyps_keep>-
+   metis_tac[sub_completion_wfs]>>
+   fs[LET_THM,EVAL``COUNT_LIST 1``]>>
+   qpat_abbrev_tac `s' = s|++ls`>>
+   first_x_assum(qspecl_then[`s'`,`menv`,
+     `(n,0,Infer_Tuvar st.next_uvar)::tenv`,
+     `st with next_uvar:= st.next_uvar+1`,`constraints'`] mp_tac)>>
+   imp_res_tac check_freevars_to_check_t>>
+   `t_wfs s'` by 
+     metis_tac[Abbr`s'`,t_wfs_eqn,extend_t_vR_WF,FUPDATE_EQ_FUPDATE_LIST]>>
+   `s SUBMAP s'` by
+     (unabbrev_all_tac>>
+     match_mp_tac SUBMAP_FUPDATE_LIST_NON_EXIST>>
+     fs[MAP_ZIP,LENGTH_COUNT_LIST]>>
+     fs[INTER_DEF,MEM_MAP,MEM_COUNT_LIST,EXTENSION]>>
+     rw[] >>DECIDE_TAC)>>
+   miscLib.discharge_hyps>>fs[]
+   >-
+     (
+     rpt strip_tac
+     >-
+       (fs[sub_completion_def]>>
+       unabbrev_all_tac>>
+       rpt strip_tac
+       >-
+         (fs[pure_add_constraints_append]>>HINT_EXISTS_TAC>>fs[]>>
+	 assume_tac pure_add_constraints_exists>>
+         pop_assum(qspecl_then [`s`,`[t1]`,`st.next_uvar`,`num_tvs tenvE`] mp_tac)>>
+	 miscLib.discharge_hyps>>
+	 fs[LET_THM,EVAL ``COUNT_LIST 1``])
+       >-
+         (fs[FDOM_FUPDATE_LIST,SUBSET_DEF]>>DECIDE_TAC)
+       >-
+         cheat)
+     >-
+       (fs[SUBSET_DEF]>>rw[]>>res_tac>>DECIDE_TAC)
+     >-
+       (unabbrev_all_tac>>
+       fs[FDOM_FUPDATE_LIST,EXTENSION]>>DECIDE_TAC)
+     >-
+       (fs[tenv_inv_def,lookup_tenv_def]>>rpt strip_tac>>
+       Cases_on`n=x`>>fs[deBruijn_inc0]
+       >-
+         (HINT_EXISTS_TAC>>fs[])
+       >- res_tac)
+     >-
+       (fs[tenv_inv_def,lookup_tenv_def]>>rpt strip_tac>>
+       Cases_on`n=x`>>fs[deBruijn_inc0]
+       >-
+       (fs[t_walkstar_eqn,t_walk_eqn,Once t_vwalk_eqn]>>
+       unabbrev_all_tac>>
+       fs[flookup_fupdate_list]>>
+       Cases_on`unconvert_t t'`
+       >-
+         fs[]
+       >-
+         (fs[MAP_EQ_ID,check_t_def,EVERY_MEM]>>rw[]>>
+	 res_tac>>metis_tac[t_walkstar_no_vars])
+       >- fs[check_t_def])
+       >>
+       res_tac>>
+       Q.EXISTS_TAC `t''`>>
+       `t_walkstar s t'' = t_walkstar s' t''` by 
+         (imp_res_tac t_walkstar_SUBMAP>>
+	 first_x_assum(qspec_then `t''` SUBST1_TAC)>>
+	 Cases_on`tvs>0`>>
+	 metis_tac[check_freevars_to_check_t,t_walkstar_no_vars])>>
+       fs[]))
+   >>
+   (strip_tac>>rw[success_eqns]>>
+   HINT_EXISTS_TAC>>HINT_EXISTS_TAC>>
+   fs[]>> CONJ_TAC
+   >- 
+     metis_tac[SUBMAP_TRANS]
+   >>
+     `t_wfs s''` by
+       (`t_wfs st''.subst` by  
+         (imp_res_tac infer_e_wfs>>
+	 rfs[])>>
+       metis_tac[sub_completion_wfs])>>
+     simp[Once t_walkstar_eqn,Once t_walk_eqn,SimpRHS]>>
+     simp[convert_t_def]>>
+     assume_tac t_walkstar_SUBMAP>>
+     pop_assum (qspecl_then [`s'`,`s''`,`Infer_Tuvar st.next_uvar`] mp_tac)>>
+     `t_walkstar s' (Infer_Tuvar st.next_uvar) = unconvert_t t1` by
+       (
+       simp[t_walkstar_eqn,t_walk_eqn,Once t_vwalk_eqn]>>
+       unabbrev_all_tac>>
+       simp[flookup_fupdate_list]>>
+       Cases_on`unconvert_t t1`
+       >-
+         simp[]
+       >-
+         (fs[MAP_EQ_ID,check_t_def,EVERY_MEM]>>rw[]>>
+	 res_tac>>metis_tac[t_walkstar_no_vars])
+       >- fs[check_t_def])>>
+     metis_tac[check_freevars_empty_convert_unconvert_id,t_walkstar_no_vars]))
+ >-
+   (*App*)
+   first_x_assum(qspecl_then [`s`,`menv`,`tenv`,`st`,`constraints`] assume_tac)>>rfs[]>>
+   Q.EXISTS_TAC `t''`>>Q.EXISTS_TAC`st''`>>
+   `constrain_op op ts' st' = (Success t'',st'')` by cheat >>
+   fs[
+   simp[PULL_EXISTS]
+   
+   fs[type_op_def]
+ >- (*Log*)
+   cheat
+ >- (*If *)
+   cheat
+ >- (*Mat*)
+   cheat
+ >- (*Let*)
+   (last_x_assum(qspecl_then [`s`,`menv`,`tenv`,`st`,`constraints`] assume_tac)>>
+   rfs[]>>
+   Cases_on `n`>>fs[opt_bind_def]
+   >-
+     (first_x_assum(qspecl_then [`s'`,`menv`,`tenv`,`st'`,`constraints'`] assume_tac)>>
+     rfs[opt_bind_tenv_def]>>
+     `t_wfs st'.subst` by 
+       imp_res_tac infer_e_wfs>>
+     imp_res_tac sub_completion_wfs>>
+     imp_res_tac tenv_inv_submap>>fs[]>>
+     ntac 2 HINT_EXISTS_TAC>>
+     fs[]>>metis_tac[SUBMAP_TRANS])
+   >>
+     cheat) (*Rest of this should be about the same as Fun*)
+ >-
+   (*Letrec*)
+   (imp_res_tac type_funs_distinct>>
+   `MAP (\x,y,z. x) funs = MAP FST funs` by
+     fs[MAP_EQ_f,FORALL_PROD]>>
+   fs[bind_var_list_def]>>
+   qpat_abbrev_tac `new_tenv = A ++ tenv`>>
+   (*last_x_assum (qspecl_then [`s',`menv`,`st with next_uvar:=st.next_uvar + LENGTH funs`,*)
+   cheat)  
  >> cheat)
  
  (*(`tenv_inv (bind n (0,Infer_Tuvar st.next_uvar) tenv) (bind_tenv n 0 t1 tenvE)`
